@@ -5,7 +5,10 @@ import Xv6.ProofMappages
 
 namespace Xv6
 
-/-- `mappages` meets its specification, given `walk`'s. -/
+/-- `mappages` meets its general (uncounted) specification, given `walk`'s. -/
+theorem MappagesAny (W : WALK) : MAPPAGES_ANY := mappages_any_proof W
+
+/-- `mappages` meets its counted specification, given `walk`'s. -/
 theorem Mappages (W : WALK) : MAPPAGES := mappages_proof W
 
 end Xv6
